\documentclass{article}
\usepackage[utf8]{inputenc}
\usepackage{url,amsmath,graphicx,amssymb,booktabs}

\title{MA3676 - Stochastic Models}
\author{Luke Dando}
\date{\today}

\begin{document}

\maketitle

\tableofcontents

\section{Sums}

\begin{enumerate}
    \item \textbf{Geometric:} 
    \begin{equation}
        1+r+r^2+r^3+\ldots=\sum_{x=0}^\infty r^x = \frac{1}{1-r},\quad |r|<1.
    \end{equation}
    
    \item \textbf{Binomial:}
    \begin{equation}
        \sum_{x=0}^n \begin{pmatrix} n\\x \end{pmatrix}p^x q^{n-x} = (p+q)^n.
    \end{equation}
    
    \item \textbf{Exponential:}
    \begin{equation}
        \sum_{x=0}^\infty \frac{\lambda^x}{x!}=e^\lambda.
    \end{equation}
    Note: $e^\lambda=\lim_{n\rightarrow\infty}(1+\frac{\lambda}{n})^n$.
\end{enumerate}

\section{Generating Functions}

A generating function $G$ on a distribution $X$ with respect to $s$ is defined as:
\begin{equation}
    G_X(s)=\mathbb{E}[s^X]=\sum_np_ns^n,\quad p_n=\mathbb{P}[X=n].
\end{equation}
It is important to note :
\begin{itemize}
    \item $ G_X(1)=1 $,
    \item $ G_X(0)=\mathbb{P}[X=0]$,
    \item $\mathbb{E}[X]=G_X^\prime(1)$,
    \item $G_{X+Y}(s)=G_X(s)G_Y(s)$.
\end{itemize}

\begin{enumerate}
    \item \textbf{Bernoulli:}
    \begin{align}
        G_X(s)=\sum_{n=0}^1 s^np_n &= s^0\cdot (1-p)+s^1\cdot(p),\quad p_n=\mathbb{P}[X=n], \\
        &=1+(s-1)p.
    \end{align}
    
    \item \textbf{Geometric:}
    \begin{align}
        G_X(s) = \sum_{n=1}^\infty s^n(1-p)^{n-1}&=(1-p)s\sum_{n=1}^\infty (sp)^{n-1}, \\
        &=(1-p)s\sum_{k=0}^\infty (sp)^{k},\quad k=n-1, \\
        &=(1-p)s \cdot \frac{1}{1-sp}, \\
        &=\frac{(1-p)s}{1-sp}.
    \end{align}
    
    \item \textbf{Binomial:} $Y_n=\sum_{i=1}^n I_n$, where $I_n$ are steps of 0 or 1, with probabilities of $p$ and $q=1-p$ respectively.
    \begin{align}
        G_{Y_n}(s) = \mathbb{E}[s^{Y_n}]&=\mathbb{E}[s^{\sum_{i=1}^\infty I_n}], \\
        &=\mathbb{E}[s^{I_1}\cdot s^{I_2} \ldots s^{I_n}], \\
        &=\mathbb{E}\left[\prod_{i=1}^n s^{I_n}\right], \\
        &=\prod_{i=1}^n\mathbb{E}[s^{I_n}], \\
        &=\prod_{i=1}^n(ps+q) = (ps+q)^n, \\
        &= \sum_{m=0}^n \begin{pmatrix} n\\m \end{pmatrix}(ps)^m(q)^{n-m}.
    \end{align}
    \item \textbf{Poisson:} Let $\mathbb{P}[X=x]=\frac{\lambda^x e^{-\lambda}}{x!}$,
    \begin{align}
        G_x(s)&=\sum_{x=0}^\infty s^x\frac{\lambda^x}{x!}e^{-\lambda}, \\
        &=e^{-\lambda}\sum_{x=0}^\infty \frac{(\lambda s)^x}{x!}, \\
        &=e^{-\lambda}e^{\lambda s}, \\
        &= e^{\lambda(s-1)}.
    \end{align}
\end{enumerate}

\end{document}
